CC: Substitutions wip

Semantic/CC/Substitution.lean
@@ -5,6 +5,7 @@ namespace CC
 structure Subst (s1 s2 : Sig) where
   var : BVar s1 .var -> Var .var s2
   tvar : BVar s1 .tvar -> Ty .shape s2
+  cvar : BVar s1 .cvar -> CaptureSet s2
 
 def Subst.lift (s : Subst s1 s2) : Subst (s1,,k) (s2,,k) where
   var := fun x => by
@@ -15,6 +16,10 @@ def Subst.lift (s : Subst s1 s2) : Subst (s1,,k) (s2,,k) where
     cases x
     case here => exact .tvar .here
     case there x => exact (s.tvar x).rename Rename.succ
+  cvar := fun x => by
+    cases x
+    case here => exact .cvar (.bound .here)
+    case there x => exact (s.cvar x).rename Rename.succ
 
 def Subst.liftMany (s : Subst s1 s2) (K : Sig) : Subst (s1 ++ K) (s2 ++ K) :=
   match K with
@@ -24,24 +29,39 @@ def Subst.liftMany (s : Subst s1 s2) (K : Sig) : Subst (s1 ++ K) (s2 ++ K) :=
 def Subst.id {s : Sig} : Subst s s where
   var := fun x => .bound x
   tvar := fun x => .tvar x
+  cvar := fun x => .cvar (.bound x)
 
 def Var.subst : Var .var s1 -> Subst s1 s2 -> Var .var s2
 | .bound x, s => s.var x
 | .free n, _ => .free n
+
+def CaptureSet.subst : CaptureSet s1 -> Subst s1 s2 -> CaptureSet s2
+| .empty, _ => .empty
+| .union cs1 cs2, σ => .union (cs1.subst σ) (cs2.subst σ)
+| .var x, σ => .var (x.subst σ)
+| .cvar x, σ => match x with
+  | .bound x => σ.cvar x
+  | .free n => .cvar (.free n)
 
 def Ty.subst : Ty sort s1 -> Subst s1 s2 -> Ty sort s2
 | .top, _ => .top
 | .tvar x, s => s.tvar x
 | .arrow T1 T2, s => .arrow (T1.subst s) (T2.subst s.lift)
 | .poly T1 T2, s => .poly (T1.subst s) (T2.subst s.lift)
+| .capt cs T, s => .capt (cs.subst s) (T.subst s)
+| .exi T, s => .exi (T.subst s.lift)
+| .typ T, s => .typ (T.subst s)
 
 def Exp.subst : Exp s1 -> Subst s1 s2 -> Exp s2
 | .var x, s => .var (x.subst s)
 | .abs T e, s => .abs (T.subst s) (e.subst s.lift)
 | .tabs T e, s => .tabs (T.subst s) (e.subst s.lift)
+| .cabs e, s => .cabs (e.subst s.lift)
 | .app x y, s => .app (x.subst s) (y.subst s)
 | .tapp x T, s => .tapp (x.subst s) (T.subst s)
+| .capp x cs, s => .capp (x.subst s) (cs.subst s)
 | .letin e1 e2, s => .letin (e1.subst s) (e2.subst s.lift)
+| .unpack e1 e2, s => .unpack (e1.subst s) (e2.subst s.lift.lift)
 
 def Subst.openVar (x : Var .var s) : Subst (s,x) s where
   var := fun
@@ -49,6 +69,8 @@ def Subst.openVar (x : Var .var s) : Subst (s,x) s where
     | .there x0 => .bound x0
   tvar := fun
     | .there x0 => .tvar x0
+  cvar := fun
+    | .there x0 => .cvar (.bound x0)
 
 def Subst.openTVar (U : Ty .shape s) : Subst (s,X) s where
   var := fun
@@ -56,16 +78,24 @@ def Subst.openTVar (U : Ty .shape s) : Subst (s,X) s where
   tvar := fun
     | .here => U
     | .there x => .tvar x
+  cvar := fun
+    | .there x => .cvar (.bound x)
 
 /-!
 Function extensionality principle for substitutions.
 -/
 theorem Subst.funext {σ1 σ2 : Subst s1 s2}
   (hvar : ∀ x, σ1.var x = σ2.var x)
-  (htvar : ∀ x, σ1.tvar x = σ2.tvar x) :
+  (htvar : ∀ x, σ1.tvar x = σ2.tvar x)
+  (hcvar : ∀ x, σ1.cvar x = σ2.cvar x) :
   σ1 = σ2 := by
   cases σ1; cases σ2
-  aesop
+  simp only [Subst.mk.injEq]
+  constructor
+  · funext x; exact hvar x
+  constructor
+  · funext x; exact htvar x
+  · funext x; exact hcvar x
 
 /-!
 Composition of substitutions.
@@ -73,6 +103,7 @@ Composition of substitutions.
 def Subst.comp (σ1 : Subst s1 s2) (σ2 : Subst s2 s3) : Subst s1 s3 where
   var := fun x => (σ1.var x).subst σ2
   tvar := fun x => (σ1.tvar x).subst σ2
+  cvar := fun x => (σ1.cvar x).subst σ2
 
 theorem Subst.lift_there_var_eq {σ : Subst s1 s2} {x : BVar s1 .var} :
   (σ.lift (k:=k)).var (.there x) = (σ.var x).rename Rename.succ := by
@@ -131,6 +162,19 @@ theorem Var.weaken_subst_comm_liftMany {x : Var .var (s1 ++ K)} {σ : Subst s1 s
         congr
     | free n => simp [Var.subst, Var.rename]
 
+theorem CaptureSet.weaken_subst_comm_liftMany {cs : CaptureSet (s1 ++ K)} {σ : Subst s1 s2} :
+  (cs.subst (σ.liftMany K)).rename ((Rename.succ (k:=k0)).liftMany K) =
+  (cs.rename (Rename.succ.liftMany K)).subst (σ.lift (k:=k0).liftMany K) := by
+  induction cs with
+  | empty => rfl
+  | union cs1 cs2 ih1 ih2 =>
+    simp [CaptureSet.subst, CaptureSet.rename, ih1, ih2]
+  | var x =>
+    simp [CaptureSet.subst, CaptureSet.rename]
+    exact Var.weaken_subst_comm_liftMany
+  | cvar x =>
+    sorry
+
 theorem Ty.weaken_subst_comm {T : Ty sort (s1 ++ K)} {σ : Subst s1 s2} :
   (T.subst (σ.liftMany K)).rename ((Rename.succ (k:=k0)).liftMany K) =
     (T.rename (Rename.succ.liftMany K)).subst (σ.lift.liftMany K) := by
@@ -147,6 +191,17 @@ theorem Ty.weaken_subst_comm {T : Ty sort (s1 ++ K)} {σ : Subst s1 s2} :
     have ih2 := Ty.weaken_subst_comm (T:=T2) (σ:=σ) (K:=K,X) (k0:=k0)
     simp [Ty.subst, Ty.rename, ih1]
     exact ih2
+  | .capt cs T =>
+    have ihT := Ty.weaken_subst_comm (T:=T) (σ:=σ) (K:=K) (k0:=k0)
+    have ihCS := CaptureSet.weaken_subst_comm_liftMany (cs:=cs) (σ:=σ) (K:=K) (k0:=k0)
+    simp [Ty.subst, Ty.rename, ihT, ihCS]
+  | .exi T =>
+    have ih := Ty.weaken_subst_comm (T:=T) (σ:=σ) (K:=K,C) (k0:=k0)
+    simp [Ty.subst, Ty.rename]
+    exact ih
+  | .typ T =>
+    have ih := Ty.weaken_subst_comm (T:=T) (σ:=σ) (K:=K) (k0:=k0)
+    simp [Ty.subst, Ty.rename, ih]
 
 theorem Ty.weaken_subst_comm_base {T : Ty sort s1} {σ : Subst s1 s2} :
   (T.subst σ).rename (Rename.succ (k:=k)) = (T.rename Rename.succ).subst (σ.lift (k:=k)) :=
@@ -157,6 +212,23 @@ theorem Var.weaken_subst_comm_base {x : Var .var s1} {σ : Subst s1 s2} :
   cases x with
   | bound x => rfl
   | free n => rfl
+
+theorem CaptureSet.weaken_subst_comm_base {cs : CaptureSet s1} {σ : Subst s1 s2} :
+  (cs.subst σ).rename (Rename.succ (k:=k)) = (cs.rename Rename.succ).subst (σ.lift) := by
+  induction cs with
+  | empty => rfl
+  | union cs1 cs2 ih1 ih2 =>
+    simp [CaptureSet.subst, CaptureSet.rename, ih1, ih2]
+  | var x =>
+    simp [CaptureSet.subst, CaptureSet.rename]
+    exact Var.weaken_subst_comm_base
+  | cvar x =>
+    cases x with
+    | bound x =>
+      simp [CaptureSet.subst, CaptureSet.rename, Var.rename, Subst.lift]
+      sorry
+    | free n =>
+      simp [CaptureSet.subst, CaptureSet.rename, Var.rename]
 
 /-!
 Composition of substitutions commutes with lifting.
@@ -181,6 +253,12 @@ theorem Subst.comp_lift {σ1 : Subst s1 s2} {σ2 : Subst s2 s3} {k : Kind} :
         lhs; simp only [Subst.comp, Subst.lift_there_tvar_eq]
       simp only [Subst.lift_there_tvar_eq]
       simp only [Ty.weaken_subst_comm_base, Subst.comp]
+  · intro C
+    cases C with
+    | here => rfl
+    | there C0 =>
+      simp [Subst.comp, Subst.lift]
+      exact CaptureSet.weaken_subst_comm_base.symm
 
 /-!
 Composition of substitutions commutes with lifting many levels.
@@ -203,6 +281,22 @@ theorem Var.subst_comp {x : Var .var s1} {σ1 : Subst s1 s2} {σ2 : Subst s2 s3}
   | bound x => rfl
   | free n => rfl
 
+theorem CaptureSet.subst_comp {cs : CaptureSet s1} {σ1 : Subst s1 s2} {σ2 : Subst s2 s3} :
+  (cs.subst σ1).subst σ2 = cs.subst (σ1.comp σ2) := by
+  induction cs with
+  | empty => rfl
+  | union cs1 cs2 ih1 ih2 =>
+    simp [CaptureSet.subst, ih1, ih2]
+  | var x =>
+    simp [CaptureSet.subst]
+    exact Var.subst_comp
+  | cvar x =>
+    cases x with
+    | bound x =>
+      simp [CaptureSet.subst, Subst.comp]
+    | free n =>
+      simp [CaptureSet.subst]
+
 /-!
 Substituting a composition of substitutions is the same as
 substituting one after the other for a type.
@@ -216,6 +310,12 @@ theorem Ty.subst_comp {T : Ty sort s1} {σ1 : Subst s1 s2} {σ2 : Subst s2 s3} :
     simp [Ty.subst, ih1, ih2, Subst.comp_lift]
   | poly T1 T2 ih1 ih2 =>
     simp [Ty.subst, ih1, ih2, Subst.comp_lift]
+  | capt cs T ih =>
+    simp [Ty.subst, ih, CaptureSet.subst_comp]
+  | exi T ih =>
+    simp [Ty.subst, ih, Subst.comp_lift]
+  | typ T ih =>
+    simp [Ty.subst, ih]
 
 /-!
 Substituting a composition of substitutions is the same as
@@ -229,9 +329,15 @@ theorem Exp.subst_comp {e : Exp s1} {σ1 : Subst s1 s2} {σ2 : Subst s2 s3} :
     simp [Exp.subst, Ty.subst_comp, ih_e, Subst.comp_lift]
   | tabs T e ih_e =>
     simp [Exp.subst, Ty.subst_comp, ih_e, Subst.comp_lift]
+  | cabs e ih_e =>
+    simp [Exp.subst, ih_e, Subst.comp_lift]
   | app x y => simp [Exp.subst, Var.subst_comp]
   | tapp x T => simp [Exp.subst, Var.subst_comp, Ty.subst_comp]
+  | capp x cs =>
+    simp [Exp.subst, Var.subst_comp, CaptureSet.subst_comp]
   | letin e1 e2 ih1 ih2 =>
+    simp [Exp.subst, ih1, ih2, Subst.comp_lift]
+  | unpack e1 e2 ih1 ih2 =>
     simp [Exp.subst, ih1, ih2, Subst.comp_lift]
 
 end CC
